Anomaly Universe Top.40279 undefined. Please report at http://coq.inria.fr/bugs/.

bedrock2/src/Examples/lightbulb.v
@@ -8,6 +8,43 @@ Local Open Scope string_scope. Local Open Scope Z_scope. Local Open Scope list_s
 Local Coercion literal (z : Z) : expr := expr.literal z.
 Local Coercion var (x : String.string) : expr := expr.var x.
 
+Definition recvEthernet :=
+    let info : varname := "info" in
+    let rxunused : varname := "rx_unused" in
+    let rx_status : varname := "rx_status" in
+    let rx_packet : varname := "rx_packet" in
+    let c : varname := "c" in
+    let len_bytes : varname := "len_bytes" in
+    let len_words : varname := "len_words" in
+    let word : varname := "word" in
+    let lan9250_readword : varname := "lan9250_readword" in
+
+    let r : varname := "r" in
+    ("recvEthernet", ((rx_packet::nil), (r::nil), bedrock_func_body:(
+        (* len rx_packet is [(MAX_ETHERNET+3) / 4] *)
+
+        (* Read RX_FIFO_INF *)
+        io! info = lan9250_readword(constr:(Ox"7C"));
+        rxunused = ((info >> constr:(16)) & ((constr:(1) << constr:(8)) - constr:(1)));
+        require (rxunused - constr:(0)) else { r = (constr:(-1)) };
+
+        (* Read Status FIFO Port *)
+        io! rx_status = lan9250_readword(constr:(Ox"40"));
+        len_bytes = (rx_status >> constr:(16) & ((constr:(1) << constr:(14)) - constr:(1)));
+        len_words = (len_bytes + (constr:(4) - constr:(1)) >> constr:(2));
+
+        (* len_words <= MAX_ETHERNET *)
+        require (len_words < constr:(1518 + 1)) else { r = (constr:(-1)) };
+
+        c = (constr:(0));
+        word = (constr:(0));
+        while (c < len_words) {
+            io! word = lan9250_readword(constr:(0));
+            store(rx_packet + c * constr:(4), word);
+            c = (c + constr:(1))
+        }
+    ))).
+
 Definition lightbulb :=
     let packet : varname := "packet" in
     let len : varname := "len" in
@@ -47,6 +84,17 @@ From bedrock2.Map Require Import Separation SeparationLogic.
 
 Local Infix "*" := sep.
 Local Infix "*" := sep : type_scope.
+
+
+
+Instance spec_of_recvEthernet : spec_of "recvEthernet" := fun functions =>
+  forall p_addr (rx_packet:list byte) R m t,
+    (array scalar8 (word.of_Z 1) p_addr rx_packet * R) m ->
+    1518 < Z.of_nat (List.length rx_packet) ->
+    (* comment on wormhole mentions < 0x400 for lan9250_readword. TODO check against manual *)
+    WeakestPrecondition.call functions "recvEthernet" t m [p_addr]
+      (fun t' m' rets => exists v, rets = [v]).
+
 Instance spec_of_lightbulb : spec_of "lightbulb" := fun functions =>
   forall p_addr packet len R m t,
     (array scalar8 (word.of_Z 1) p_addr packet * R) m ->
@@ -65,6 +113,119 @@ Ltac seplog_use_array_load1 H i :=
 (* TODO why does typeclass search fail here? *)
 Local Instance mapok: map.ok mem := SortedListWord.ok (Naive.word 32 eq_refl) _.
 Local Instance wordok: word.ok word := coqutil.Word.Naive.ok _ _.
+
+Lemma recvEthernet_ok : program_logic_goal_for_function! recvEthernet.
+Proof.
+  repeat straightline.
+
+  seplog_use_array_load1 H 0.
+  seplog_use_array_load1 H 64.
+  seplog_use_array_load1 H 124.
+  repeat straightline.
+
+  cbn [args ext_spec FE310CSemantics.parameters].
+  do 2 eexists; split. { eapply Properties.map.split_empty_r. reflexivity. }
+  split; [cbv; clear; intuition congruence | intros].
+  repeat straightline.
+  exists m. split. { eapply Properties.map.split_empty_r. reflexivity. }
+  repeat straightline.
+
+  (* if for early out *)
+  letexists; split; repeat straightline; split; [|repeat straightline; eauto].
+  repeat straightline.
+
+
+  cbn [args ext_spec FE310CSemantics.parameters].
+  do 2 eexists; split. { eapply Properties.map.split_empty_r. reflexivity. }
+  split; [cbv; clear; intuition congruence | intros].
+  repeat straightline.
+  exists m. split. { eapply Properties.map.split_empty_r. reflexivity. }
+  repeat straightline.
+
+  letexists; split; repeat straightline; split; [|repeat straightline; eauto].
+  repeat straightline.
+
+  (* while loop *)
+  refine (TailRecursion.tailrec
+    (* types of ghost variables*) HList.polymorphic_list.nil
+    (* program variables *) ["info";"rx_unused";"rx_status";"rx_packet";"c";"len_bytes";"len_words";"word"]
+    (fun v t m info rx_unused rx_status rx_packet c len_bytes len_words_loop word => 
+        PrimitivePair.pair.mk (v = word.unsigned c /\
+        exists scratch R, (array scalar8 (word.of_Z 1) (word.add rx_packet (word.mul c (word.of_Z 4)) )  scratch * R) m /\
+        Z.of_nat (List.length scratch) = word.unsigned (word.mul (word.sub len_words c) (word.of_Z 4) ) /\
+        len_words_loop = len_words)  (* precondition *)
+    (fun   T M INFO RX_UNUSED RX_STATUS RX_PACKET C LEN_BYTES LEN_WORDS WORD => (* postcondition *) True))
+    (fun n m : Z => m < n <= word.unsigned len_words) (* well_founded relation *)
+    _ _ _ _ _);
+    (* TODO wrap this into a tactic with the previous refine *)
+    cbn [HList.hlist.foralls HList.tuple.foralls
+         HList.hlist.existss HList.tuple.existss
+         HList.hlist.apply  HList.tuple.apply
+         HList.hlist
+         List.repeat Datatypes.length
+         HList.polymorphic_list.repeat HList.polymorphic_list.length
+         PrimitivePair.pair._1 PrimitivePair.pair._2] in *.
+
+  { repeat straightline. }
+  { exact (Z.gt_wf _). }
+  { repeat straightline. eauto. 1:admit. }
+  { repeat straightline.  cbn [args ext_spec FE310CSemantics.parameters].
+    do 2 eexists; split. { eapply Properties.map.split_empty_r. reflexivity. }
+    split; [cbv; clear; intuition congruence | intros].
+    repeat straightline.
+    eexists. split. { eapply Properties.map.split_empty_r. eauto. }
+
+  repeat straightline.
+  apply Properties.word.if_nonzero in H6.
+  rewrite word.unsigned_ltu in H6.
+  rewrite Z.ltb_lt in H6.
+
+  rewrite <- (List.firstn_skipn 4 x7) in H7.
+Require Import coqutil.Macros.symmetry.
+   SeparationLogic.seprewrite_in (symmetry! @bytearray_index_merge) H7.
+
+  { rewrite List.length_firstn_inbounds. { instantiate (1:= word.of_Z 4). eauto. }
+  apply Znat.Nat2Z.inj_le.
+  rewrite H8. revert H6. admit. }
+
+  eapply store_word_of_sep. { 
+    revert H10. unfold scalar. unfold truncated_scalar. unfold littleendian. unfold ptsto_bytes.ptsto_bytes. admit. (* this needs to be proven to fill in H7, scratch *)}
+  { 
+  
+  do 6 straightline.
+  (* TODO more than 6 straightlines takes too long *)
+
+    Import Markers.hide.
+    do 8 letexists. split. 
+    { repeat straightline. }
+    { letexists. split.
+    { split. { repeat straightline. }
+             { letexists. 
+               { repeat straightline. letexists. 
+                 { split. {
+  replace (word.add
+             (word.add x2 (word.mul x3 (word.of_Z 4)))
+             (word.of_Z 4)) with (word.add x2 (word.mul c (word.of_Z 4))) in H10.
+  { ecancel_assumption. }
+  { subst c. (* TODO ring. *) admit. }}
+
+  assert (scratch=(List.skipn 4 x7)). { repeat straightline. }
+  { repeat straightline. subst scratch. rewrite List.length_skipn. subst c.
+  rewrite Znat.Nat2Z.inj_sub.
+  { rewrite H8. (* ring *) admit. }
+  (* same as apply Znat.Nat2Z.inj_le admitted above  *) admit. }}}}}
+  repeat straightline. split.
+  { subst v3. subst v'. subst c. admit. }
+  repeat straightline. }}}
+   repeat straightline. (* Coq anomaly *)
+
+}}}} 
+
+
+
+
+
+Admitted.
 
 (* bsearch.v has examples to deal with arrays *)
 Lemma lightbulb_ok : program_logic_goal_for_function! lightbulb.
@@ -116,4 +277,5 @@ Proof.
   clear. eauto.
 Qed.
 
+Compute BasicCSyntax.c_func (recvEthernet).
 Compute BasicCSyntax.c_func (lightbulb).
